linear_coq/LinearRule.v
@@ -1,6 +1,6 @@
 Require Import Metalib.Metatheory.
 Require Import Program.Equality.
-(* Require Import PositiveBase. *)
+Require Import Rules.
 
 
 Module M.
