linear_coq/infra.v
@@ -1,0 +1,515 @@
+Require Import Metalib.Metatheory.
+Require Import Program.Equality.
+Require Export Rules.
+
+Ltac destruct_hypos :=
+  repeat
+    match goal with
+    | [H : _ /\ _ |- _ ] => destruct H
+    | [H : exists _, _ |- _ ] => destruct H              
+    end.
+
+
+Lemma decide_typ : forall x y : typ, {x = y} + {~ x = y}.
+  intros.
+  decide equality.
+  decide equality.
+Defined.
+
+Lemma subst_tt_intro_rec : forall X T2 U k,
+  X `notin` fv_tt T2 ->
+  open_tt_rec k U T2 = subst_tt X U (open_tt_rec k (typ_fvar X) T2).
+Proof with congruence || auto.
+  induction T2; intros U k Fr; simpl in *; f_equal...
+
+    destruct (k === n)... simpl. destruct (X == X)...
+
+    destruct (a == X)... contradict Fr; fsetdec.
+Qed.
+
+Lemma subst_tt_intro : forall X T2 U,
+  X `notin` fv_tt T2 ->
+  open_tt T2 U = subst_tt X U (open_tt T2 X).
+Proof.
+  intros.
+  unfold open_tt.
+  apply subst_tt_intro_rec...
+  assumption.
+Qed.
+
+Lemma open_tt_rec_type_aux : forall T j V i U,
+  i <> j ->
+  open_tt_rec j V T = open_tt_rec i U (open_tt_rec j V T) ->
+  T = open_tt_rec i U T.
+Proof with congruence || eauto.
+  induction T; intros j V i U Neq H; simpl in *; inversion H; f_equal...
+    destruct (j === n)... destruct (i === n)...
+Qed.
+
+Lemma open_tt_rec_type : forall T U k,
+  type T ->
+  T = open_tt_rec k U T.
+Proof with auto.
+  intros T U k Htyp. revert k.
+  induction Htyp; intros k; simpl; f_equal...
+
+    unfold open_tt in *.
+    pick fresh X.
+    apply open_tt_rec_type_aux with (j:=0) (V:=X).
+    auto.
+    auto.
+Qed.
+
+Lemma subst_tt_fresh : forall Z U T,
+   Z `notin` fv_tt T ->
+   T = subst_tt Z U T.
+Proof with auto.
+  induction T; simpl; intro H; f_equal...
+
+    destruct (a == Z)...
+    contradict H; fsetdec.
+Qed.
+    
+Lemma subst_tt_open_tt_rec : forall T1 T2 X P k,
+  type P ->
+  subst_tt X P (open_tt_rec k T2 T1) =
+    open_tt_rec k (subst_tt X P T2) (subst_tt X P T1).
+Proof with auto.
+  intros T1 T2 X P k WP. revert k.
+  induction T1; intros k; simpl; f_equal...
+
+    destruct (k === n); subst...
+
+    destruct (a == X); subst... apply open_tt_rec_type...
+Qed.
+
+Lemma subst_tt_open_tt : forall T1 T2 (X:atom) P,
+  type P ->
+  subst_tt X P (open_tt T1 T2) = open_tt (subst_tt X P T1) (subst_tt X P T2).
+Proof with auto.
+  intros.
+  unfold open_tt.
+  apply subst_tt_open_tt_rec...
+Qed.
+
+Lemma subst_tt_open_tt_var : forall (X Y:atom) P T,
+  Y <> X ->
+  type P ->
+  open_tt (subst_tt X P T) Y = subst_tt X P (open_tt T Y).
+Proof with congruence || auto.
+  intros X Y P T Neq Wu.
+  unfold open_tt.
+  rewrite subst_tt_open_tt_rec...
+  simpl.
+  destruct (Y == X)...
+Qed.
+
+Lemma subst_tt_type : forall Z P T,
+  type T ->
+  type P ->
+  type (subst_tt Z P T).
+Proof with auto.
+  intros Z P T HT HP.
+  induction HT; simpl...
+
+  destruct (X == Z)...
+
+    pick fresh Y and apply type_mu...
+    rewrite subst_tt_open_tt_var...
+Qed.
+
+Lemma open_ee_rec_expr_aux : forall e j v u i,
+  i <> j ->
+  open_ee_rec j v e = open_ee_rec i u (open_ee_rec j v e) ->
+  e = open_ee_rec i u e.
+Proof with congruence || eauto.
+  induction e; intros j v u i Neq H; simpl in *; inversion H; f_equal...
+
+    destruct (j===n)... destruct (i===n)...
+Qed.
+
+
+Lemma open_ee_rec_expr : forall u e k,
+  expr e ->
+  e = open_ee_rec k u e.
+Proof with auto.
+  intros u e k Hexpr. revert k.
+  induction Hexpr; intro k; simpl; f_equal; auto*;
+  try solve [
+    unfold open_ee in *;
+    pick fresh x;
+    eapply open_ee_rec_expr_aux with (j := 0) (v := exp_fvar x);
+    auto
+  | unfold open_te in *;
+    pick fresh X;
+    eapply open_ee_rec_type_aux with (j := 0) (V := typ_fvar X);
+    auto
+  ].
+Qed.
+
+Lemma subst_ee_fresh : forall (x: atom) u e,
+  x `notin` fv_exp e ->
+  e = subst_ee x u e.
+Proof with auto.
+  intros x u e; induction e; simpl; intro H; f_equal...
+
+    destruct (a==x)...
+    contradict H; fsetdec.
+Qed.
+
+Lemma subst_ee_open_ee_rec : forall e1 e2 x u k,
+  expr u ->
+  subst_ee x u (open_ee_rec k e2 e1) =
+    open_ee_rec k (subst_ee x u e2) (subst_ee x u e1).
+Proof with auto.
+  intros e1 e2 x u k WP. revert k.
+  induction e1; intros k; simpl; f_equal...
+
+    destruct (k === n); subst...
+
+    destruct (a == x); subst... apply open_ee_rec_expr...
+Qed.
+
+Lemma subst_ee_open_ee : forall e1 e2 x u,
+  expr u ->
+  subst_ee x u (open_ee e1 e2) =
+    open_ee (subst_ee x u e1) (subst_ee x u e2).
+Proof with auto.
+  intros.
+  unfold open_ee.
+  apply subst_ee_open_ee_rec...
+Qed.
+
+Lemma subst_ee_open_ee_var : forall (x y:atom) u e,
+  y <> x ->
+  expr u ->
+  open_ee (subst_ee x u e) y = subst_ee x u (open_ee e y).
+Proof with congruence || auto.
+  intros x y u e Neq Wu.
+  unfold open_ee.
+  rewrite subst_ee_open_ee_rec...
+  simpl.
+  destruct (y == x)...
+Qed.
+
+
+Lemma subst_ee_intro_rec : forall x e u k,
+  x `notin` fv_exp e ->
+  open_ee_rec k u e = subst_ee x u (open_ee_rec k (exp_fvar x) e).
+Proof with congruence || auto.
+  induction e; intros u k Fr; simpl in *; f_equal...
+
+    destruct (k === n)... simpl. destruct (x == x)...
+
+    destruct (a == x)... contradict Fr; fsetdec.
+Qed.
+
+Lemma subst_ee_intro : forall x e u,
+  x `notin` fv_exp e ->
+  open_ee e u = subst_ee x u (open_ee e x).
+Proof with auto.
+  intros.
+  unfold open_ee.
+  apply subst_ee_intro_rec...
+Qed.
+
+
+(* ================================================ *)
+(* ================================================ *)
+(* ================================================ *)
+(* ================================================ *)
+(* ================================================ *)
+(* ================================================ *)
+
+
+Lemma In_lemmaR : forall {X: Type} (E1:list X) A  E2,
+    In A E2 -> In A (E1 ++ E2).
+Proof.
+  induction E1; intros. simpl. auto.
+  rewrite <- app_comm_cons.
+  apply in_cons.
+  apply  IHE1.
+  assumption.
+Qed.  
+
+Lemma In_lemmaL : forall {X: Type}  E2 (E1:list X) A,
+    In A E1 -> In A ( E1 ++ E2).
+Proof.
+  induction E2;intros.
+  -
+    rewrite app_nil_r.
+    assumption.
+  -
+    rewrite cons_app_one.
+    rewrite <- app_assoc.
+    apply IHE2.
+    apply in_split in H.
+    destruct H.
+    destruct H.
+    rewrite H.
+    rewrite app_assoc.
+    apply In_lemmaR.
+    rewrite cons_app_one.
+    rewrite app_assoc.
+    rewrite <-cons_app_one.
+    apply in_eq.
+Qed.
+
+
+
+Lemma wfs_type: forall E T,
+    WFS E T -> type T.
+Proof with auto.
+  intros.
+  induction H...
+  apply type_mu with (L:=L)...
+Qed.
+
+Lemma subst_open_tt_rec : forall T A, type A -> forall Y X,
+    Y `notin` fv_tt T ->
+    X `notin` fv_tt T -> forall n,
+        subst_tt X Y (open_tt_rec n A T) = open_tt_rec n (subst_tt X Y A) T.
+Proof with auto.
+  induction T; intros; unfold open_tt in *; simpl in *; try solve [f_equal;eauto]; eauto.
+  - destruct (n0 == n); simpl; eauto.
+  - destruct (a == X); simpl; eauto; subst.
+    apply notin_singleton_1 in H1.
+    destruct H1...
+Qed.
+
+
+Lemma wfs_weakening: forall E1 E2 T E,
+    WFS (E1 ++ E2) T ->
+    WFS (E1 ++ E ++ E2) T.
+Proof with auto.
+  intros.
+  generalize dependent E.
+  dependent induction H;intros...
+  -
+    apply WFS_fvar with (im:=im)...
+  -
+    apply WFS_rec with (L:=L) (im:=im)...
+    intros.
+    rewrite_alist (([(X, bind_sub im)] ++ E1) ++ E ++ E2).
+    apply H0...
+Qed.
+
+Lemma subst_tt_wfs: forall A B E X,
+    WFS E A ->
+    WFS E B ->
+    WFS E (subst_tt X A B).
+Proof with auto.
+  intros.
+  generalize dependent A.
+  dependent induction H0;intros...
+  -
+    simpl.
+    destruct (X0==X)...
+    apply WFS_fvar with (im:=im)...
+  -
+    simpl in *...
+  -
+    simpl.
+    apply WFS_rec with (L:=L \u {{X}} \u fv_tt A0) (im:=im)...
+    intros.
+    rewrite subst_tt_open_tt_var...
+    apply H0...
+    rewrite_alist (nil ++ [(X0, bind_sub im)] ++ E).
+    apply wfs_weakening...
+    apply wfs_type with (E:=E)...
+Qed.
+
+Lemma notin_fv_subst: forall X A B Y,
+    X \notin fv_tt A ->
+    X \notin fv_tt B ->
+    X <> Y ->
+    X \notin fv_tt (subst_tt Y A B).
+Proof with auto.
+  intros.
+  induction B;simpl in *...
+  destruct (a == Y)...
+Qed.
+
+Lemma notin_union: forall X A B,
+    X `notin` (union A B) <->
+    X `notin` A /\ X `notin` B.
+Proof.
+  intros.
+  split.
+  split; auto.
+  intros.
+  destruct H.
+  auto.  
+Qed.
+
+
+Lemma notin_fv_tt_open_aux : forall X U T,
+    X `notin` fv_tt T ->
+    X \notin fv_tt U ->
+    X `notin` fv_tt (open_tt T U).
+Proof with auto.
+  intros.
+  simpl.
+  unfold open_tt.
+  unfold open_tt_rec.
+  generalize 0.
+  induction T;simpl in *;intros...
+  destruct (n0==n)...
+Qed.
+
+Lemma in_dec: forall T X,
+    X \notin T \/ X \in T.
+Proof with auto.
+  intros.
+  apply notin_diff_1.
+  assert (AtomSetImpl.diff T T [=] Metatheory.empty).
+  apply AtomSetProperties.diff_subset_equal.
+  apply KeySetProperties.subset_refl.
+  rewrite H...
+Qed.
+
+Lemma in_open: forall A X Y,
+    X `in` fv_tt A ->
+    X <> Y ->
+    X `in` fv_tt (open_tt A Y).
+Proof with auto.
+  intros A X Y.
+  unfold open_tt.
+  generalize 0.
+  induction A;intros;simpl in *...
+  apply AtomSetProperties.FM.empty_iff in H.
+  destruct H.
+  apply AtomSetImpl.union_1 in H.
+  destruct H.
+  apply AtomSetImpl.union_2.
+  apply IHA1...
+  apply AtomSetImpl.union_3.
+  apply IHA2...
+Qed.
+
+Lemma open_rec_eq :
+  forall A1 A2 X n,
+    open_tt_rec n (typ_fvar X) A1 = open_tt_rec n X A2 ->
+    X \notin (union (fv_tt A1) (fv_tt A2)) ->
+    A1 = A2.
+Proof with auto.
+  induction A1; intros; simpl in *.
+  -
+    destruct A2; simpl in *; try (inversion H); eauto.
+    destruct (n == n0); inversion H.
+  - destruct A2; simpl in *; try (inversion H); eauto.
+    destruct (n == n0); inversion H.
+  - destruct (n0 == n).
+    destruct A2; simpl in *; try (inversion H); eauto.
+    destruct (n0 == n1); subst; eauto.
+    inversion H. subst.
+    apply notin_union in H0.
+    destruct H0.
+    apply notin_singleton_1 in H1.
+    destruct H1...
+    destruct A2; simpl in *; try (inversion H); eauto.
+    destruct (n0 == n2); try (inversion H).
+    subst. eauto.
+  - destruct A2; simpl in *; try (inversion H); eauto.
+    destruct (n == n0); try (inversion H).
+    apply notin_union in H0.
+    destruct H0.
+    apply notin_singleton_1 in H0.
+    destruct H0...
+  - destruct A2; simpl in *; try (inversion H); eauto.
+    destruct (n == n0); inversion H.
+    apply IHA1 in H2; eauto. rewrite H2.
+    eauto.
+  - destruct A2; simpl in *; try (inversion H); eauto.
+    destruct (n == n0); inversion H.
+    apply IHA1_1 in H2; eauto.
+    apply IHA1_2 in H3; eauto.
+    subst. eauto.
+Qed.
+
+Lemma in_open0: forall A X Y k,
+    X `in` fv_tt (open_tt_rec k A Y) ->
+    X `in` fv_tt A \/ X \in fv_tt Y.
+Proof with auto.
+  intros.
+  generalize dependent k.
+  induction Y;intros;simpl in *...
+  -
+    destruct (k==n)...
+  -
+    specialize (IHY (S k)).
+    apply IHY in H.
+    destruct H...
+  -
+    apply AtomSetImpl.union_1 in H. 
+    destruct H.
+    specialize (IHY1 k).
+    apply IHY1 in H.
+    destruct H...
+    specialize (IHY1 k).
+    apply IHY2 in H.
+    destruct H...
+Qed.
+
+Lemma in_open1: forall A X Y ,
+    X `in` fv_tt (open_tt Y A) ->
+    X `in` fv_tt A \/ X \in fv_tt Y.
+Proof with auto.
+  intros.
+  unfold open_tt in *.
+  apply in_open0 with (k:=0)...
+Qed.
+
+  
+
+Lemma in_notin: forall T X Y,
+    X \in T ->
+          Y \notin T ->
+          X <> Y.
+Proof with auto.
+  intros.
+  apply AtomSetProperties.add_equal in H.  
+  rewrite AtomSetProperties.add_union_singleton in H.
+  rewrite <- H in H0.
+  auto.
+Qed.
+(* 
+Lemma subst_tt_wfs2: forall A B E1 E2 X im,
+    WFS (E1 ++ E2) A ->
+    WFS (E1 ++ (X ~ bind_sub im) ++ E2) B ->
+    WFS (E1 ++ E2) (subst_tt X A B).
+Proof with auto.
+  intros.
+  generalize dependent A.
+  dependent induction H0;intros...
+  -
+    simpl.
+    destruct (X0==X)...
+    apply WFS_fvar with (im:=im0)...
+    analyze_binds H...
+    
+  -
+    simpl in *...
+    apply WFS_arrow.
+    apply IHWFS1 with (im:=im)...
+  -
+    simpl.
+    apply WFS_rec with (L:=L \u {{X}} \u fv_tt A0).
+    intros.
+    rewrite <- subst_open_unfoldn...
+    rewrite_alist (([(X0, bind_sub)] ++ E1) ++ E2).
+    apply H0...
+    rewrite_alist (nil ++ [(X0, bind_sub)] ++ (E1 ++ E2)).
+    apply wfs_weakening...
+    apply wfs_type with (E:=E1 ++ E2)...
+Qed. *)
+
+
+Ltac solve_notin :=
+  repeat
+    match goal with
+    | [H : _ |- _ \notin fv_tt (open_tt _ _) ] => apply notin_fv_tt_open_aux
+    | [H : _ |- _ \notin fv_tt (subst_tt _ _ _) ] => apply notin_fv_subst
+    | [H : _ |- _ \notin (_ \u _) ] => apply notin_union;split
+    | [H : _ |- _ \notin _ ] => simpl;auto               
+    end.
